Algorithm Correctness Done

Rocq/src/Algo.v
@@ -1,4 +1,7 @@
 From Stdlib Require Import Lists.List.
+From Stdlib Require Import Arith.Compare_dec.
+From Stdlib Require Import PeanoNat.
+From Stdlib Require Import Logic.FunctionalExtensionality.
 
 From Verilog Require Import Expr.
 From Verilog Require Import ExprPath.
@@ -8,8 +11,8 @@ From Verilog Require Import TypeSystem.
 From Verilog Require Import Spec.
 From Verilog Require Import Utils.
 
+Import Nat.
 Import ListNotations.
-
 
 Import Path.
 Import Expr.
@@ -19,6 +22,7 @@ Import TypedExprPath.
 Import TypeSystem.
 Import Spec.
 Import Utils.
+Import Learn.
 
 Module Algo.
   Fixpoint down s e :=
@@ -26,174 +30,241 @@ Module Algo.
     | TAtom _ op => TAtom s op
     | TBinOp _ tLhs tRhs => TBinOp s (down s tLhs) (down s tRhs)
     | TUnOp _ tArg => TUnOp s (down s tArg)
-    | TCast _ tArg => TCast s tArg
-    | TComp _ tLhs tRhs => TComp s tLhs tRhs
-    | TLogic _ tLhs tRhs => TLogic s tLhs tRhs
-    | TReduction _ tArg => TReduction s tArg
-    | TShift _ tLhs tRhs => TShift s (down s tLhs) tRhs
-    | TAssign _ lval tArg => TAssign s lval tArg
-    | TShiftAssign _ lval tArg => TShiftAssign s lval tArg
-    | TCond _ tArg tLhs tRhs => TCond s tArg (down s tLhs) (down s tRhs)
-    | TConcat _ tArgs => TConcat s tArgs
-    | TRepl _ n tArg => TRepl s n tArg
+    | TCast _ tArg => TCast s (down (size tArg) tArg)
+    | TComp _ tLhs tRhs =>
+        let sArg := max (size tLhs) (size tRhs) in
+        TComp s (down sArg tLhs) (down sArg tRhs)
+    | TLogic _ tLhs tRhs => TLogic s (down (size tLhs) tLhs) (down (size tRhs) tRhs)
+    | TReduction _ tArg => TReduction s (down (size tArg) tArg)
+    | TShift _ tLhs tRhs => TShift s (down s tLhs) (down (size tRhs) tRhs)
+    | TAssign _ lval tArg =>
+        let sArg := max lval (size tArg) in
+        TAssign s lval (down sArg tArg)
+    | TShiftAssign _ lval tArg => TShiftAssign s lval (down (size tArg) tArg)
+    | TCond _ tArg tLhs tRhs => TCond s (down (size tArg) tArg) (down s tLhs) (down s tRhs)
+    | TConcat _ tArgs =>
+        TConcat s (map (fun tE => down (size tE) tE) tArgs)
+    | TRepl _ n tArg => TRepl s n (down (size tArg) tArg)
     end
   .
-
-  Definition down_curry (x: nat * TypedExpr) := let (s, e) := x in down s e.
 
   Fixpoint up e :=
     match e with
-    | EAtom op => (op, TAtom op op)
+    | EAtom op => TAtom op op
     | EBinOp lhs rhs =>
-        let (lhsS, uLhs) := up lhs in
-        let (rhsS, uRhs) := up rhs in
-        let s := max lhsS rhsS in
-        (s, TBinOp s uLhs uRhs)
+        let uLhs := up lhs in
+        let uRhs := up rhs in
+        let s := max (size uLhs) (size uRhs) in
+        TBinOp s uLhs uRhs
     | EUnOp arg =>
-        let (argS, uArg) := up arg in
-        (argS, TUnOp argS uArg)
+        let uArg := up arg in
+        TUnOp (size uArg) uArg
     | ECast arg =>
-        let (argS, uArg) := up arg in
-        let dArg := down argS uArg in
-        (argS, TUnOp argS dArg)
+        let uArg := up arg in
+        TCast (size uArg) uArg
     | EComp lhs rhs =>
-        let (lhsS, uLhs) := up lhs in
-        let (rhsS, uRhs) := up rhs in
-        let s := max lhsS rhsS in
-        let dLhs := down s uLhs in
-        let dRhs := down s uRhs in
-        (1, TComp 1 dLhs dRhs)
+        let uLhs := up lhs in
+        let uRhs := up rhs in
+        TComp 1 uLhs uRhs
     | ELogic lhs rhs =>
-        let (lhsS, uLhs) := up lhs in
-        let (rhsS, uRhs) := up rhs in
-        let dLhs := down lhsS uLhs in
-        let dRhs := down rhsS uRhs in
-        (1, TLogic 1 dLhs dRhs)
+        let uLhs := up lhs in
+        let uRhs := up rhs in
+        TLogic 1 uLhs uRhs
     | EReduction arg =>
-        let (argS, uArg) := up arg in
-        let dArg := down argS uArg in
-        (1, TReduction 1 dArg)
+        let uArg := up arg in
+        TReduction 1 uArg
     | EShift lhs rhs =>
-        let (lhsS, uLhs) := up lhs in
-        let (rhsS, uRhs) := up rhs in
-        let dRhs := down rhsS uRhs in
-        (lhsS, TLogic lhsS uLhs dRhs)
+        let uLhs := up lhs in
+        let uRhs := up rhs in
+        TShift (size uLhs) uLhs uRhs
     | EAssign lval arg =>
-        let (argS, uArg) := up arg in
-        let s := max lval argS in
-        let dArg := down s uArg in
-        (lval, TAssign lval lval dArg)
+        let uArg := up arg in
+        TAssign lval lval uArg
     | EShiftAssign lval arg =>
-        let (argS, uArg) := up arg in
-        let dArg := down argS uArg in
-        (lval, TAssign lval lval dArg)
+        let uArg := up arg in
+        TShiftAssign lval lval uArg
     | ECond arg lhs rhs =>
-        let (argS, uArg) := up arg in
-        let (lhsS, uLhs) := up lhs in
-        let (rhsS, uRhs) := up rhs in
-        let s := max lhsS rhsS in
-        let dArg := down argS uArg in
-        (s, TCond s dArg uLhs uRhs)
+        let uArg := up arg in
+        let uLhs := up lhs in
+        let uRhs := up rhs in
+        let s := max (size uLhs) (size uRhs) in
+        TCond s uArg uLhs uRhs
     | EConcat args =>
         let uArgs := map up args in
-        let dArgs := map down_curry uArgs in
-        let s := sum (map fst uArgs) in
-        (s, TConcat s dArgs)
+        let s := sum (map size uArgs) in
+        TConcat s uArgs
     | ERepl n arg =>
-        let (argS, uArg) := up arg in
-        let dArg := down argS uArg in
-        let s := n * argS in
-        (s, TReduction s dArg)
+        let uArg := up arg in
+        TReduction (n * (size uArg)) uArg
     end
   .
 
-  Definition type e := down_curry (up e).
+  Definition type e := let tE := up e in down (size tE) tE.
 
   Definition size_at e p := option_map size (e @@[p]).
 
-  Theorem down_shape : forall e p s, IsTypedPath e p <-> IsTypedPath (down s e) p.
+  Lemma down_shape1 : forall e p, IsTypedPath e p -> forall s, IsTypedPath (down s e) p.
   Proof.
-    split; intros.
-    - induction H; simpl in *; econstructor; eassumption.
-    - generalize dependent p. induction e; intros; simpl in *;
-        try (inv H; constructor; firstorder).
-      inv H0. constructor. econstructor; eassumption.
+    intros. generalize dependent s. induction H; intros; simpl in *;
+      econstructor; firstorder.
+      rewrite nth_error_map. rewrite H. reflexivity.
   Qed.
 
-  Theorem up_shape : forall e p, IsPath e p <-> IsTypedPath (snd (up e)) p.
+  Lemma down_shape2 : forall e p s, IsTypedPath (down s e) p -> IsTypedPath e p.
+  Proof.
+    induction e; intros; try (inv H; constructor; firstorder).
+    inv H0. constructor. destruct (nth_error args n) eqn:Hnth;
+      rewrite nth_error_map in H3; rewrite Hnth in H3; inv H3.
+    econstructor. eassumption. apply (H _ _ Hnth _ _ H5).
+  Qed.
+
+  Theorem down_shape : forall e p, IsTypedPath e p <-> forall s, IsTypedPath (down s e) p.
   Proof.
     split; intros.
-    Ltac _up_shape :=
-      match goal with
-      | [ |- IsTypedPath (snd (let (_, _) := up ?e in _)) _ ] => destruct (up e)
-      | [ H: IsTypedPath (snd (let (_, _) := up ?e in _)) _ |- _ ] => destruct (up e)
-      | [ H: IsTypedPath (down _ _) _ |- _ ] => rewrite <- down_shape in H
-      end
-    .
-    - induction H; simpl in *; repeat _up_shape; simpl in *; try constructor;
-        try (apply down_shape); try assumption.
+    - apply (down_shape1 _ _ H).
+    - apply (down_shape2 _ _ 0 (H _)).
+  Qed.
+
+  Theorem up_shape : forall e p, IsPath e p <-> IsTypedPath (up e) p.
+  Proof.
+    split; intros.
+    - induction H; simpl in *; simpl in *; try (constructor; assumption).
       econstructor.
-      + repeat (rewrite nth_error_map). rewrite H. simpl in *. reflexivity.
-      + destruct (up e). simpl in *. apply down_shape. assumption.
-    - generalize dependent p. induction e; intros; simpl in *; repeat _up_shape;
-        simpl in *; try (inv H); try constructor; repeat _up_shape; try firstorder.
-      inv H0.
-      + constructor.
-      + repeat (rewrite nth_error_map in H3). destruct (nth_error args n) eqn:HArg;
-        inv H3. econstructor.
-        * eassumption.
-        * eapply H. eassumption. destruct (up e0). simpl in *.
-          rewrite <- down_shape in H5. assumption.
+      + rewrite nth_error_map. rewrite H. reflexivity.
+      + assumption.
+    - generalize dependent p. induction e; intros; simpl in *;
+        try (inv H; constructor; firstorder).
+      inv H0. constructor. destruct (nth_error args n) eqn:Hnth;
+        rewrite nth_error_map in *; rewrite Hnth in *; inv H3. econstructor.
+      + eassumption.
+      + firstorder.
   Qed.
 
   Theorem type_shape : forall e p, IsPath e p <-> IsTypedPath (type e) p.
   Proof.
-    intros. unfold type. destruct (up e) eqn:Hup. simpl. rewrite <- down_shape.
-    assert (Ht: t = snd (up e)) by (rewrite Hup; reflexivity). subst. apply up_shape.
+    split; intros; unfold type in *.
+    - rewrite up_shape in H. apply (down_shape1 _ _ H _).
+    - apply up_shape. apply (down_shape2 _ _ _ H).
   Qed.
 
-  Hint Unfold type : core.
-  Hint Unfold size_at : core.
-  Hint Unfold down_curry : core.
-
-  Theorem up_size : forall e, fst (up e) = determine e.
+  Lemma up_top_size : forall e, size (up e) = determine e.
   Proof.
-    Ltac _up_size :=
-      match goal with
-      | [ |- fst (let (_, _) := up ?e in _) = _ ] => destruct (up e)
-      | [ H: fst (up ?e) = _ |- _ ] => destruct (up e)
-      end
-    .
-    induction e using Expr_ind; autounfold; simpl;
-      repeat _up_size; simpl in *; try congruence.
+    induction e using Expr_ind; simpl; firstorder.
     induction args.
     - reflexivity.
-    - simpl. rewrite (H 0 _ (eq_refl _)). rewrite IHargs.
-      + reflexivity.
-      + intros n. apply (H (S n)).
+    - simpl. rewrite (H 0). rewrite IHargs. reflexivity. intros n.
+      apply (H (S n)). reflexivity.
   Qed.
 
-  Theorem down_size : forall e s, size (down s e) = s.
+  Lemma down_top_size : forall e s, size (down s e) = s.
   Proof.
-    intros [] ?; reflexivity.
+    intros; destruct e; reflexivity.
   Qed.
 
-  Theorem type_size : forall e, size (type e) = determine e.
+  Lemma type_top_size : forall e, size (type e) = determine e.
   Proof.
-    intros. autounfold. destruct (up e) eqn:Hup.
-    assert (fst (up e) = n) by (rewrite Hup; reflexivity).
-    rewrite down_size. rewrite <- H. apply up_size.
+    intros. unfold type. rewrite up_top_size. apply down_top_size.
   Qed.
 
-  Theorem ttoreike : forall e t f,
-      e ==> t -| f -> forall p, IsPath e p -> size_at (type e) p = f p.
+  Theorem up_size_path : forall e p, size_at (up e) p = option_map determine (e @[p]).
   Proof.
-    intros. induction p using path_ind.
-    - unfold size_at. rewrite sub_typed_expr_nil. simpl. rewrite type_size.
-      destruct (synth_must_be_determine H). congruence.
-    - unfold size_at. admit.
-  Admitted.
+    intros; unfold size_at; destruct (IsPath_dec e p).
+    - assert (HpTe: IsTypedPath (up e) p) by (apply up_shape; assumption).
+      induction i; try (inv HpTe; firstorder).
+      + rewrite sub_expr_nil. rewrite sub_typed_expr_nil. simpl.
+        rewrite up_top_size. reflexivity.
+      + simpl. rewrite H3. rewrite nth_error_map in H3. rewrite H in *. inv H3.
+        firstorder.
+    - assert (Hse: e @[p] = None). {
+          destruct (e @[p]) eqn:Hse.
+          - exfalso. apply n. apply (sub_expr_valid _ _ _ Hse).
+          - reflexivity.
+      }
+      assert (HsTe: up e @@[p] = None). {
+        destruct (up e @@[p]) eqn:HsTe.
+        - exfalso. apply n. apply sub_typed_expr_valid in HsTe.
+          rewrite <- up_shape in HsTe. assumption.
+        - reflexivity.
+      }
+      rewrite Hse. rewrite HsTe. reflexivity.
+  Qed.
+
+  Ltac inv_path :=
+    match goal with
+    | [ H: IsPath (_ _) _ |- _ ] => inv H
+    end
+  .
+
+  Lemma down_size_path_lemma :
+    forall e s fc, e <== s -| fc -> forall p, IsPath e p -> fc p = size_at (down s (up e)) p.
+  Proof.
+    Ltac _down_size_dec :=
+      match goal with
+      | [ |- _ = option_map _ (down (max ?n ?m) _ @@[_]) ] =>
+          let nH := fresh in destruct (max_dec_bis n m) as [[nH ?]|[nH ?]];
+                             rewrite nH in *; clear nH
+      end
+    .
+    Ltac _down_size_p_lem :=
+      match goal with
+      | [ H: _ = _ |- _ ] => rewrite <- H
+      | [ H: _ -> _ |- _ ] => eapply H; eassumption
+      | [ H: _ ==> _ -| _ |- _ ] =>
+          learn (synth_must_be_determine _ _ _ H); splitHyp; subst
+      | [ H: ?e ==> determine ?e -| _ |- _ ] =>
+          learn (synth_can_check _ _ _ _ H (le_refl _)); existsHyp
+      | [ H: ?e ==> ?t -| ?f1, F: ?e <== ?t -| ?f2 |- _ ] =>
+          let nH := fresh in assert (nH: f1 = f2) by
+            (extensionality p; apply (synth_check_inj_f _ _ _ _ H F));
+                             learn nH; subst
+      | [ H: ?e1 ==> ?t -| _, F: ?e2 <== ?t -| _ |- _ ] =>
+          learn (synth_check_determine_order _ _ _ _ _ _ H F (le_refl _));
+          try antisym; subst
+      | [ H: ?e <== ?t -| _, F: ?t <= determine ?e |- _ ] =>
+          learn (synth_and_order _ _ _ H F); subst
+      end
+    .
+    induction e using Expr_ind; intros; simpl in *; unfold size_at; inv_path;
+      try (apply check_root in H; simpl; congruence);
+      inv_ts; simpl; repeat (rewrite up_top_size);
+      try _down_size_dec; repeat _down_size_p_lem; try lia; try reflexivity.
+    repeat (gen_nth). repeat (rewrite nth_error_map). rewrite H3. rewrite H0. simpl.
+    repeat (rewrite up_top_size). specialize (H8 _ _ _ _ H3 H1 H0).
+    repeat _down_size_p_lem.
+  Qed.
+
+  Theorem down_size_path : forall e s,
+      determine e <= s -> e <== s -| size_at (down s (up e)).
+  Proof.
+    intros. destruct (always_synth e) as [t [f Hs]].
+    destruct (synth_must_be_determine _ _ _ Hs). subst. clear H1.
+    destruct (synth_can_check _ _ _ _ Hs H) as [fc Hc]. clear Hs. clear f.
+    assert (Hfc: fc = size_at (down s (up e))).
+    {
+      extensionality p.
+      destruct (fc p) eqn:Hfc.
+      - assert (Hp: IsPath e p) by (rewrite (check_f_path _ _ _ Hc); exists n; assumption).
+        rewrite <- Hfc. apply down_size_path_lemma; assumption.
+      - assert (Hp: ~(IsTypedPath (down s (up e)) p)).
+        { unfold not. intros. apply down_shape2 in H0. rewrite <- up_shape in H0.
+          rewrite (check_f_path _ _ _ Hc) in H0. destruct H0. congruence. }
+        unfold size_at. destruct (down s (up e) @@[ p]) eqn:HsTe.
+        + exfalso. apply Hp. apply (sub_typed_expr_valid _ _ _ HsTe).
+        + reflexivity.
+    }
+    rewrite <- Hfc. assumption.
+  Qed.
+
+  Theorem toto: forall e, exists t, e ==> t -| size_at (type e).
+  Proof.
+    intros. exists (determine e). destruct (always_synth e) as [t [f Hs]].
+    destruct (synth_must_be_determine _ _ _ Hs); subst.
+    assert (Hc: e <== determine e -| size_at (type e)).
+    { unfold type. rewrite up_top_size. apply down_size_path. reflexivity. }
+    assert (Hf: f = size_at (type e))
+      by (extensionality p; apply (synth_check_inj_f _ _ _ _ Hs Hc)).
+    subst. assumption.
+  Qed.
 
 End Algo.
-
 
