Rocq/src/Extr.v
@@ -1,0 +1,16 @@
+From Stdlib Require Import PeanoNat.
+From Stdlib Require Import Extraction.
+
+From Verilog Require Import Algo.
+Import Algo.
+
+Extraction Language OCaml.
+Set Extraction Output Directory ".".
+
+Extract Inductive list => "list" [ "[]" "(::)" ].
+Extract Inductive nat => "int" [ "0" "succ" ].
+
+Extract Constant Nat.add => "( + )".
+Extract Constant Nat.mul => "( * )".
+Extract Constant Nat.max => "(fun x y -> max x y)".
+
